work in progress: change subnode without trans, btnode induction principle, and eventually relation predicate to link abstract iterators to btrees

verif/db/verif_operations.v
@@ -1,185 +1,501 @@
 Require Import VST.floyd.proofauto.
-Require Import Signatures.
-Require Import db_operations.
-
-Require btrees.btrees. Require btrees.btrees_sep. 
-
-
-Instance CompSpecs : compspecs. make_compspecs prog. Defined.
-Definition Vprog : varspecs. mk_varspecs prog. Defined.
-
-Require Import FiniteSet FlatData SortedTuples SortedAttributes Values Plans.
-
+Require Import VST.floyd.library.
+Require Import VST.msl.iter_sepcon.
+Require Signatures.
+Require btrees.btrees.
+Require btrees.btrees_sep. Require btrees.btrees_spec.
+Require FiniteSet FlatData SortedTuples SortedAttributes Values Plans.
 Require SeqScan.
+Require db_operations.
 
-Fixpoint string_to_list_byte (s: string) : list byte :=
-  match s with
-  | EmptyString => nil
-  | String a s' => Byte.repr (Z.of_N (Ascii.N_of_ascii a)) :: string_to_list_byte s'
-  end.
+Section Tuple.
+  Import Values SortedAttributes FiniteSet FlatData Plans.
+  Fixpoint string_to_list_byte (s: string) : list byte :=
+    match s with
+    | EmptyString => nil
+    | String a s' => Byte.repr (Z.of_N (Ascii.N_of_ascii a)) :: string_to_list_byte s'
+    end.
 
-Definition stringpool : Type := (* This is only temporary. *)
-  { v | (type_of_value v) = type_string } -> val.
+  Definition stringpool : Type := (* This is only temporary. *)
+    { v | (type_of_value v) = type_string } -> val.
 
-Program Definition val_of_value (sp : stringpool) (v : value) : val :=
-  match v with
-  | Value_string s => sp (exist _ v _)
-  | Value_ptrofs x => Vint (Ptrofs.to_int x) end.
+  Program Definition val_of_value (sp : stringpool) (v : value) : val :=
+    match v with
+    | Value_string s => sp (exist _ v _)
+    | Value_ptrofs x => Vint (Ptrofs.to_int x) end.
 
-(* This need to be implemented. *)
-Definition stringpool_rep (sp : stringpool) : mpred := emp.
+  (* This need to be implemented. *)
+  Definition stringpool_rep (sp : stringpool) : mpred := emp.
 
-Definition tuple := Tuple1.tuple attribute value OAN FAN.
-Definition support := Tuple1.support attribute value OAN FAN.
-Definition dot := Tuple1.dot attribute value OAN FAN.
+  Definition tuple := Tuple.tuple TPL.T.
+  Definition support : tuple -> setA := Tuple.support TPL.T.
+  Definition attribute := Tuple.attribute TPL.T.
+  Definition dot : tuple -> attribute -> value := Tuple.dot TPL.T. Check dot.
+  Definition Otuple : OrderedSet.Oeset.Rcd tuple := Tuple.OTuple TPL.T.
+  Global Opaque tuple support attribute dot Otuple.
 
-Definition tuple_rep (sh : share) (t : tuple) (p : val) : mpred :=
-  EX sp : stringpool,
-          data_at sh (tarray size_t (Z.of_nat (Fset.cardinal FAN (support t))))
-                  (map (val_of_value sp oo dot t) (Fset.elements FAN (support t))) p * stringpool_rep sp.
+  Definition tuple_rep (sh : share) (t : tuple) (p : val) : mpred :=
+    EX sp : stringpool,
+            data_at sh (tarray size_t (Z.of_nat (Fset.cardinal FAN (support t))))
+                    (map (val_of_value sp oo dot t) ({{{support t}}})) p * stringpool_rep sp.
+End Tuple. 
 
-Definition t_attr_list_t := Tstruct _attribute_list_t noattr.
+Section CompSpecs.
+  
+  Definition db_operations_CompSpecs : compspecs. make_compspecs db_operations.prog. Defined.
+  Definition db_operations_Vprog : varspecs. mk_varspecs db_operations.prog. Defined.
 
-Definition id_of_attribute (a : attribute) : list byte :=
-  match a with
-  | Attr_string _ s => string_to_list_byte s
-  | Attr_ptrofs _ s => string_to_list_byte s end.
+  Definition relation_mem_CompSpecs : compspecs. make_compspecs relation_mem.prog. Defined.
+  Definition relation_mem_Vprog : varspecs. mk_varspecs relation_mem.prog. Defined.
+  
+End CompSpecs.
 
-Definition domain_of_attribute (a : attribute) : val :=
-  match a with
+Section AttrList.
+  Import db_operations SortedAttributes FiniteSet.
+
+  Existing Instance db_operations_CompSpecs.
+  
+  Definition t_attr_list_t := Tstruct _attribute_list_t noattr.
+  
+  Definition id_of_attribute (a : attribute) : list byte :=
+    match a with
+    | Attr_string _ s => string_to_list_byte s
+    | Attr_ptrofs _ s => string_to_list_byte s end.
+
+  Definition domain_of_attribute (a : attribute) : val :=
+    match a with
     | Attr_ptrofs _ _ => Vint (Int.repr 0)
     | Attr_string _ _ => Vint (Int.repr 1) end.
 
-Definition attribute_string_rep sh (a : attribute) (p : val) : mpred :=
-  match a with
-  | Attr_ptrofs _ _ => emp
-  | Attr_string _ s => cstring sh (string_to_list_byte s) p end.
+  Definition attribute_string_rep sh (a : attribute) (p : val) : mpred :=
+    match a with
+    | Attr_ptrofs _ _ => emp
+    | Attr_string _ s => cstring sh (string_to_list_byte s) p end.
 
-Fixpoint attribute_lseg_rep (sh : share) (l : list attribute) (p q : val) : mpred :=
-  match l with
-  | [] => !! (p = q /\ is_pointer_or_null p) && emp
-  | a :: tl =>
-    EX r : val, EX sptr : val, data_at sh t_attr_list_t (sptr, (domain_of_attribute a, r)) p * attribute_lseg_rep sh tl r q * attribute_string_rep sh a sptr end.
+  Fixpoint attribute_lseg_rep (sh : share) (l : list attribute) (p q : val) : mpred :=
+    match l with
+    | [] => !! (p = q /\ is_pointer_or_null p) && emp
+    | a :: tl =>
+      EX r : val, EX sptr : val, data_at sh t_attr_list_t (sptr, (domain_of_attribute a, r)) p * attribute_lseg_rep sh tl r q * attribute_string_rep sh a sptr end.
 
-Lemma attribute_lseg_nil sh l : attribute_lseg_rep sh l nullval nullval |-- !! (l = []).
-Proof.
-  destruct l; simpl; entailer.
-  saturate_local. apply field_compatible_nullval with (P := False) in H.
-  contradiction.
-Qed.
- 
-Definition attribute_list_rep sh l p := attribute_lseg_rep sh l p nullval.
+  Lemma attribute_lseg_nil sh l : attribute_lseg_rep sh l nullval nullval |-- !! (l = []).
+  Proof.
+    destruct l; simpl; entailer.
+    saturate_local. apply field_compatible_nullval with (P := False) in H.
+    contradiction.
+  Qed.
+  
+  Definition attribute_list_rep sh l p := attribute_lseg_rep sh l p nullval.
 
-Lemma attribute_lseg_rep_local_facts:
-  forall sh l p q,
-   attribute_lseg_rep sh l p q |--
-                      !! (is_pointer_or_null p /\ is_pointer_or_null q).
-Proof.
-  induction l; intros; unfold attribute_lseg_rep; entailer.
-  fold attribute_lseg_rep. sep_apply IHl. entailer.
-Qed.
+  Lemma attribute_lseg_rep_local_facts:
+    forall sh l p q,
+      attribute_lseg_rep sh l p q |--
+                         !! (is_pointer_or_null p /\ is_pointer_or_null q).
+  Proof.
+    induction l; intros; unfold attribute_lseg_rep; entailer.
+    fold attribute_lseg_rep. sep_apply IHl. entailer.
+  Qed.
 
-Hint Resolve attribute_lseg_rep_local_facts : saturate_local.
+  Hint Resolve attribute_lseg_rep_local_facts : saturate_local.
 
-Lemma attribute_list_rep_local_facts:
-  forall sh l p,
-   attribute_list_rep sh l p |--
-                      !! (is_pointer_or_null p /\ (p=nullval <-> l=nil)).
-Proof.
-  unfold attribute_list_rep, attribute_lseg_rep. induction l; intros; entailer.
-  entailer!. easy.
-  fold attribute_lseg_rep in IHl |- *.
-  sep_apply (IHl r). entailer!. apply field_compatible_nullval1 in H0.
-  easy.
-Qed.
+  Lemma attribute_list_rep_local_facts:
+    forall sh l p,
+      attribute_list_rep sh l p |--
+                         !! (is_pointer_or_null p /\ (p=nullval <-> l=nil)).
+  Proof.
+    unfold attribute_list_rep, attribute_lseg_rep. induction l; intros; entailer.
+    entailer!. easy.
+    fold attribute_lseg_rep in IHl |- *.
+    sep_apply (IHl r). entailer!. apply field_compatible_nullval1 in H0.
+    easy.
+  Qed.
 
-Hint Resolve attribute_list_rep_local_facts : saturate_local.
+  Hint Resolve attribute_list_rep_local_facts : saturate_local.
 
-Lemma attribute_list_rep_valid_pointer:
-  forall sh l p, readable_share sh ->
-   attribute_list_rep sh l p |-- valid_pointer p.
-Proof.
-  intros.
-  unfold attribute_list_rep; destruct l; simpl. entailer.
-  Intros r sptr. sep_apply data_at_valid_ptr.
-  apply readable_nonidentity. assumption.
-  entailer.
-Qed.
+  Lemma attribute_list_rep_valid_pointer:
+    forall sh l p, readable_share sh ->
+                   attribute_list_rep sh l p |-- valid_pointer p.
+  Proof.
+    intros.
+    unfold attribute_list_rep; destruct l; simpl. entailer.
+    Intros r sptr. sep_apply data_at_valid_ptr.
+    apply readable_nonidentity. assumption.
+    entailer.
+  Qed.
 
-Hint Resolve attribute_list_rep_valid_pointer : valid_pointer.
+  Hint Resolve attribute_list_rep_valid_pointer : valid_pointer.
 
-Definition attributes_rep (sh : share) (attrs : Fset.set FAN) (p : val) : mpred :=
-  attribute_list_rep sh ({{{attrs}}}) p.
+  Definition attributes_rep (sh : share) (attrs : Fset.set FAN) (p : val) : mpred :=
+    attribute_list_rep sh ({{{attrs}}}) p.
 
-Definition attribute_list_length_spec :=
- DECLARE _attribute_list_length
-  WITH sh: share, l: val, attrs: Fset.set FAN
-  PRE [ _l OF (tptr t_attr_list_t)]
-     PROP(readable_share sh)
-     LOCAL (temp _l l; temp _x l)
-     SEP (attributes_rep sh attrs l)
-  POST [ size_t ]
-     PROP()
-     LOCAL(temp ret_temp (Vint (Int.repr (Z.of_nat (Fset.cardinal _ attrs)))))
-     SEP (attributes_rep sh attrs l).
+  Definition attribute_list_length_spec :=
+    DECLARE _attribute_list_length
+            WITH sh: share, l: val, attrs: Fset.set FAN
+                                                    PRE [ _l OF (tptr t_attr_list_t)]
+                                                    PROP(readable_share sh)
+                                                    LOCAL (temp _l l; temp _x l)
+                                                    SEP (attributes_rep sh attrs l)
+                                                    POST [ size_t ]
+                                                    PROP()
+                                                    LOCAL(temp ret_temp (Vint (Int.repr (Z.of_nat (Fset.cardinal _ attrs)))))
+                                                    SEP (attributes_rep sh attrs l).
 
-Import QEP. (* QEP.cursor --> cursor *)
 
-Definition t_iterator_t := Tstruct _iterator_t noattr.
-Definition t_methods := Tstruct _methods noattr.
-Definition t_seq_scan_env := Tstruct _seq_scan_env noattr.
-Definition t_index_join_env := Tstruct _index_join_env noattr.
+End AttrList.
 
-Local Notation O := (Tuple.OTuple TPL.T).
+Section Iterator.
+  Import db_operations FlatData Plans Signatures.
+  
+  Existing Instance db_operations_CompSpecs.
+  
+  Definition t_iterator_t := Tstruct _iterator_t noattr.
+  Definition t_methods := Tstruct _methods noattr.
+  Definition t_seq_scan_env := Tstruct _seq_scan_env noattr.
+  Definition t_index_join_env := Tstruct _index_join_env noattr.
 
-Record iterator_class (c: Cursor.Rcd O) :=
-  {
-    env: Type;
-    env_rep: env -> val -> mpred;
-    env_init: env -> env;
-    env_next: env -> env;
-    (* axioms *)
-    env_close: env -> env;
-  }.
-Arguments env {c}.
-Arguments env_init {c}.
-Arguments env_next {c}.
-Arguments env_close {c}.
-Arguments env_rep {c}.
+  Record iterator_class (c: Cursor.Rcd Otuple) :=
+    {
+      env: Type;
+      env_assert: env -> Cursor.cursor c -> val -> mpred;
+      env_init: env -> env;
+      env_next: env -> env;
+      (* +axioms *)
+      env_close: env -> env;
+    }.
+  Arguments env {c}.
+  Arguments env_assert {c}.
+  Arguments env_init {c}.
+  Arguments env_next {c}.
+  Arguments env_close {c}.
 
-Definition result_rep sh (r : result tuple) (p: val) : mpred :=
-  match r with
-  | Result t => tuple_rep sh t p
-  | No_Result => emp (* ??? *)
-  | Empty_Cursor => !! (p = nullval) end.
+  Definition result_rep sh (r : result tuple) (p: val) : mpred :=
+    match r with
+    | Result t => tuple_rep sh t p
+    | No_Result => emp (* ??? *)
+    | Empty_Cursor => !! (p = nullval) end.
 
-Definition next_spec {c: Cursor.Rcd O} (cl : iterator_class c) :=
-  WITH p: val, e: env cl, it: Cursor.cursor c, t: val, sh: share
+  Definition next_spec {c: Cursor.Rcd Otuple} (cl : iterator_class c) :=
+    WITH p: val, e: env cl, it: Cursor.cursor c, sh: share, gv: globals
   PRE [ _env OF (tptr tvoid) ]
-  PROP()
-  LOCAL(temp _env p)
-  SEP(env_rep cl e p)
+  PROP(Cursor.coherent it)
+  LOCAL(gvars gv; temp _env p)
+  SEP(mem_mgr gv; env_assert cl e it p)
   POST [ tptr tvoid ]
+  EX t: val,
   PROP()
   LOCAL(temp ret_temp t)
-  SEP(result_rep sh (fst (Cursor.next it)) t * cl.(env_rep) (cl.(env_next) e) p).
+  SEP(mem_mgr gv; result_rep sh (fst (Cursor.next it)) t; cl.(env_assert) (cl.(env_next) e) (snd (Cursor.next it)) p).
+  
+  Import btrees_sep btrees.
 
-Definition seqscan_iterator : iterator_class (SeqScan.SeqScan.build O) :=
-  {|
-    env := btrees.relation val * btrees.cursor val;
-    env_rep := fun e p =>
-                 let (rel, cur) := e in
-                 let (relnode, qrel) := rel in
-                 EX qcur: val,
+  Lemma node_dec_eq {X:Type} {h: EqDec X}: forall n1 n2: node X,
+      {n1 = n2} + {n1 <> n2}.
+  Proof.
+    fix hrec 1.
+    intros. decide equality. 
+    apply bool_dec. apply bool_dec. apply bool_dec.
+    decide equality. decide equality.
+    apply Int.eq_dec. apply Int.eq_dec.
+    apply Int.eq_dec. decide equality.
+  Qed.
+  
+  Lemma subchild_nth {X}: forall (n: node X) le, subchild n le -> exists i, nth_node_le i le = Some n.
+  Proof.
+    induction le.
+    easy.
+    intro h. inversion h. exists 0%nat. easy.
+    specialize (IHle H1). destruct IHle.
+    exists (S x)%nat.
+    easy.
+  Qed.
+  Open Scope nat_scope.
+  Lemma index_le_split_l': forall m n p, n <= m -> n <= index.max_nat m p.
+  Proof.
+    induction m; intros n p h. omega.
+    simpl. destruct p. assumption.
+    transitivity (S m). assumption.
+    apply le_n_S. apply IHm.
+    omega.
+  Qed.
+
+  Lemma index_le_r: forall n m, m <= index.max_nat n m.
+  Proof.
+    induction n.
+    simpl. easy.
+    destruct m.
+    omega.
+    simpl. apply le_n_S. apply IHn.
+  Qed.
+    
+  
+  Inductive subnode' {X : Type} : node X -> node X -> Prop :=
+    sub_refl' : forall n : node X, subnode' n n
+  | sub_ptr0' : forall (n m : node X) (le : listentry X) (First Last : bool) (x : X),
+               subnode' n m -> subnode' n (btnode X (Some m) le false First Last x)
+  | sub_child' : forall (n m : node X) (le : listentry X) (ptr0 : option (node X)) (First Last : bool) (x : X),
+      subnode' n m -> subchild m le -> subnode' n (btnode X ptr0 le false First Last x).
+
+  Definition nodeDepthOrder X (n1 n2: node X) : Prop:= (node_depth n1 < node_depth n2)%nat.
+  
+  Lemma nodeDepthOrder_wf' {X} : forall depth, forall n, (node_depth n <= depth)%nat -> Acc (nodeDepthOrder X) n.
+  Proof.
+    unfold nodeDepthOrder.
+    induction depth; intros.
+    inversion H.
+    constructor. intros. omega.
+    constructor. intros.
+    inversion H.
+    + constructor. intros. apply IHdepth. omega.
+    + apply IHdepth. omega.
+  Defined.
+
+  Theorem nodeDepthOrder_wf (X: Type) : well_founded (nodeDepthOrder X).
+    red; intro; eapply nodeDepthOrder_wf'; eauto.
+  Defined.
+  
+  Program Definition sub_trans' {X: Type}: forall n m p: node X,
+      subnode' n m -> subnode' m p -> subnode' n p := fun n m =>
+    Fix (nodeDepthOrder_wf X) (fun p => subnode' n m -> subnode' m p -> subnode' n p) _.
+  Next Obligation.
+    inversion H1.
+    rewrite H3 in H0. assumption.
+    apply sub_ptr0'.
+    refine (H m0 _ _ _).
+    unfold nodeDepthOrder.
+    rewrite <- H4. simpl.
+    apply index.le_max_split_r. omega.
+    assumption.
+    assumption.
+    apply (sub_child' _ m0). apply H.
+    unfold nodeDepthOrder.
+    rewrite <- H5. apply subchild_nth in H3. destruct H3.
+    simpl.
+    apply (Nat.lt_le_trans _ (listentry_depth le)).
+    apply (nth_node_le_decrease _ le _ x1 H3).
+    apply index_le_split_l'. omega.
+    assumption.
+    assumption.
+    assumption.
+ Defined.
+  
+  Lemma subnode_cons {X: Type} {heqdec: EqDec X} {n0} {ptr0} {k k'} {n n'} {le} {First Last} {x}
+        (h: subnode' n0 (btnode X (Some ptr0) (cons X (keychild X k' n') le) false First Last x)):
+ n0 <> (btnode X (Some ptr0) (cons X (keychild X k' n') le) false First Last x) ->
+ subnode' n0 (btnode X (Some ptr0) (cons X (keychild X k n) (cons X (keychild X k' n') le)) false First Last x).
+  Proof.
+    revert n0 h. fix hrec 1.
+    intros n0 hsubn0 hneq.
+    inversion hsubn0.
+    + easy.
+    + constructor. assumption.
+    + apply (sub_child' _ m). assumption.
+      apply sc_cons. assumption.
+  Qed.
+  
+  Lemma root_integrity_cons {X} {ptr0} {k k'} {n n'} {le} {First Last} {x}
+   (hint: root_integrity (btnode X (Some ptr0) (cons X (keychild X k n) (cons X (keychild X k' n') le)) false First Last x)):
+    root_integrity (btnode X (Some ptr0) (cons X (keychild X k' n') le) false First Last x).
+  Proof.
+    unfold root_integrity in hint |- *.
+    fix hrec 1.
+    intros n0 hn0.
+    inversion hn0.
+    ++ unfold node_integrity.
+       specialize (hint (btnode X (Some ptr0) (cons X (keychild X k n) (cons X (keychild X k' n') le)) false First Last x) (sub_refl _)).
+       inversion hint. assumption.
+    ++ apply hint.
+       constructor.
+    ++ apply hint.
+       apply sub_child.
+       apply sc_cons. assumption.
+    ++ apply hint.
+      admit. 
+Admitted.
+
+Definition btnode_induction {X} (P: node X -> Prop)
+           (hleaf: forall n, LeafNode n -> P n)
+           (hintern: forall (children: list (key * node X)) (h : children <> []) n First Last x,
+               Forall (P oo snd) children -> P n ->
+               P (btnode X (Some n)
+                         (fold_right (fun (kn : key * node X) le => let (k, n) := kn in cons X (keychild X k n) le) (nil X) children) false First Last x)) : forall n, root_integrity n -> P n.
+Proof.
+  fix hrec 1.
+  intros n rint. unfold root_integrity in rint.
+  destruct n as [[n0 |] le [] ].
+  + specialize (rint (btnode _ (Some n0) le true b b0 x) (sub_refl _)).
+    simpl in rint. easy.
+  + pose (children := listentry_rect X (fun _ => list (key * node X)) []
+                                     (fun e l acc => match e with
+                                                     | keychild k n' => (k, n') :: acc
+                                                     | _ => [] (* doesn't happen *) end) le).
+    simpl in children.
+    assert (le_not_nil: le <> nil X).
+    { intro. subst le. specialize (rint (btnode X (Some n0) (nil X) false b b0 x) (sub_refl _)).
+      easy. }
+    assert (children_not_nil: children <> []).
+    { destruct le. easy. simpl in children.
+      destruct e. specialize (rint (btnode X (Some n0) (cons X (keyval X k v x0) le) false b b0 x) (sub_refl _)). simpl in rint. inversion rint.
+      easy. }
+    replace le with (fold_right
+                       (fun (kn : key * node X) (le : listentry X) => let (k, n) := kn in cons X (keychild X k n) le)
+                       (nil X) children).
+  - apply (hintern children children_not_nil n0 b b0 x). clear le_not_nil children_not_nil.
+    rewrite Forall_forall. intros [childk childnode] hkn. simpl.
+    apply hrec. 
+    unfold root_integrity. intros subn hsubn.
+    apply rint.
+    apply sub_trans with (n1 := childnode). assumption.
+    apply sub_child.
+    apply In_nth with (d := (childk, childnode)) in hkn.
+    destruct hkn as [i [hi hnth]].
+    apply nth_subchild with (i := i).
+    subst children.
+    clear rint.
+    revert le hi hnth.
+    induction i ; destruct le.
+    ++ easy.
+    ++ destruct e. easy.
+       intros _ hnth. simpl in hnth. inversion hnth. easy.
+    ++ easy.
+    ++ simpl. destruct e. easy.
+       intros. simpl in *. apply IHi.
+       omega. easy.
+    ++ apply hrec. unfold root_integrity.
+       intros n hsn. apply rint.
+       apply sub_trans with (n2 := n0). assumption.
+       constructor.
+  - subst children. clear children_not_nil. destruct le.
+    easy. clear le_not_nil. simpl.
+    destruct e. specialize (rint _ (sub_refl _)). inversion rint.
+    revert k n rint.
+    induction le; simpl.
+    reflexivity.
+    intros k n rint.
+    destruct e. specialize (rint _ (sub_refl _)). inversion rint. inversion H0.
+    simpl in IHle. simpl. f_equal.
+    apply IHle.
+    intros n2 hn2.
+    inversion hn2.
+    ++ unfold node_integrity.
+       specialize (rint (btnode X (Some n0) (cons X (keychild X k n) (cons X (keychild X k0 n1) le)) false b b0 x) (sub_refl _)).
+       inversion rint. assumption.
+    ++ apply rint.
+       constructor.
+    ++ apply rint.
+       apply sub_child.
+       apply sc_cons. assumption.
+    ++ (* hn2 is obtained by transitivity. *)
+      
+      admit. 
+    + apply hleaf. easy.
+    + specialize (rint (btnode X None le false b b0 x) (sub_refl _)).
+      easy.
+Defined.
+
+    
+    intros n1 hn1.
+    inversion hn1.
+    simpl. specialize (rint (btnode X (Some n0) (cons X (keychild X k n) le) false b b0 x) (sub_refl _)) as rint1.
+    simpl in rint1. inversion rint1. 
+
+        
+      assert (hlenil : le <> nil X).
+      { intro hfalse. subst le. simpl in children. subst children. easy. }
+      
+      induction le.
+      ++ easy. 
+      ++ destruct e.
+         
+         pose proof (rint (btnode X (Some n0) (cons X (keyval X k0 v x0) le) false b b0 x) (sub_refl _)).
+         simpl in H0.
+         inversion H0.
+         Print sc_eq.
+         apply sc_eq.
+         simpl in hkn. destruct hkn.
+         
+         apply rint.
+      Print intern_le.
+      induction le. easy.
+      simpl in nint. inversion nint.
+      subst le. inversion H.
+      subst e. unfold In in hkn.
+      subst children. simpl in hkn.
+      
+
+
+  Lemma cursor_iter_next_abs_node {X} (r: relation X):
+    (get_numrec r > O)%nat ->
+    root_integrity (get_root r) ->
+    let c := moveToFirst (get_root r) [] 0 in
+    let l := abs_node (get_root r) in
+    forall n: nat,
+      getCKey (Nat.iter n (fun c' => RL_MoveToNext c' r) c) = option_map fst (nth_error l n).
+  Proof.
+    destruct r as [root proot]. case_eq root. intros o le isLeaf First Last x hroot. simpl.
+    intros hnempty rint.
+    assert (H : (exists n, o = Some n) \/ le <> nil X).
+    {
+      destruct o.
+      { left. exists n. reflexivity. }
+      { right. intro. subst le. unfold get_numrec in hnempty. simpl in hnempty. omega. }
+    }
+    induction n; simpl; intros; destruct isLeaf.
+    + assert (o = None /\ leaf_le le).
+      { unfold root_integrity, node_integrity in rint. specialize rint with root.
+        rewrite hroot in rint. apply rint. constructor. }
+      destruct H0. subst o. destruct H as [[] | ]. discriminate.
+      destruct le. contradiction.
+      simpl. inversion H1. subst e. simpl.
+      reflexivity.
+    + unfold root_integrity, node_integrity in rint. 
+      specialize (rint root). rewrite hroot in rint. specialize (rint (sub_refl _)).
+      destruct o; [ | easy].
+      inversion rint; subst le; clear H.
+    - simpl. Print moveToFirst.
+
+
+      
+      case_eq le; intro hle. simpl. rewrite hle in H.
+      unfold get_numrec, node_numrec in H. simpl in H. destruct o; try easy.
+      
+
+    
+  (* This predicate states that the btree and cursor physically represent
+     the abstract sequential scan iterator. *) (*
+  Definition seqscan_env_assert (bt: relation val) (c: cursor val)
+             (it: Cursor.cursor (SeqScan.SeqScan.build Otuple)) : mpred :=
+    (* The root node of the btree and its address. *)
+    let (root, pbt) := bt in
+    let l : list (tuple * val) :=
+        List.combine (Cursor.collection it) (List.map Vint (snd (List.split (abs_node relnode)))) in
+*)
+  Definition seqscan_iterator : iterator_class (SeqScan.SeqScan.build Otuple) :=
+    {|
+      env := btrees.relation val * btrees.cursor val;
+      env_assert := fun e it p =>
+                   let (rel, cur) := e in
+                   let (relnode, qrel) := rel in
+                   let l : list (tuple * val) :=
+                       List.combine (Cursor.collection it) (List.map Vint (snd (List.split (abs_node relnode)))) in
+                   EX qcur: val,
+                            !! (Forall (fun x: tuple * val => option_map Vint (getCRecord cur) = Some (snd x) ->
+                                                 fst (Cursor.next it) = Result (fst x)) l /\
+                            complete_cursor (snd e) (relnode, qrel) /\
+                                correct_depth (relnode, qrel) /\ root_wf (get_root (relnode, qrel)) /\
+                                root_wf relnode) &&
+                               iter_sepcon (fun x : tuple * val => let (t, p) := x in tuple_rep Tsh t p) l *
                                         data_at Tsh t_seq_scan_env (qrel, qcur) p *
-                                        btrees_sep.relation_rep (fst e) (btrees.get_numrec (fst e)) *
-                                        btrees_sep.cursor_rep (snd e) (fst e) qcur;
-    env_init := fun e => (fst e, btrees.moveToFirst (fst (fst e)) (snd e) 0);
-    env_next := fun e => (fst e, btrees.moveToNext (snd e) (fst e));
-    env_close := fun e => e; (* FreeRecord? *)
-  |}.
+                                        relation_rep (fst e) (btrees.get_numrec (fst e)) *
+                                        cursor_rep (snd e) (fst e) qcur;
+      env_init := fun e => (fst e, btrees.moveToFirst (fst (fst e)) (snd e) 0);
+      env_next := fun e => (fst e, btrees.moveToNext (snd e) (fst e));
+                             env_close := fun e => e; (* FreeRecord? *)
+       (* +axioms *)
+    |}.
+  
+  Definition seqscan_next_spec := (DECLARE _seq_scan_next (next_spec seqscan_iterator)).
+End Iterator.
 
-Definition seqscan_next_spec := (DECLARE _seq_scan_next (next_spec seqscan_iterator)).
 
 (* MATERIALIZE: WORK IN PROGRESS
 Definition materialize_spec :=
@@ -191,46 +507,90 @@ Definition materialize_spec :=
     SEP(iterator_rep sh c it)
     POST [  *)
 
-Definition Gprog := ltac:(with_library prog [attribute_list_length_spec; seqscan_next_spec]).
 
-Lemma body_seqscan_next: semax_body Vprog Gprog f_seq_scan_next seqscan_next_spec.
-Proof.
-  unfold seqscan_next_spec, next_spec.
-  start_function.
-  simpl env_rep.
-  destruct e as [rel c], rel as [relnode qrel].
-  Intros qcur.
-  forward.
-Admitted.  
-
-Lemma body_attribute_list_length: semax_body Vprog Gprog f_attribute_list_length attribute_list_length_spec.
-Proof.
-  start_function.
-  forward. forward.
-  forward_loop
-    (EX x : val, EX l1 : list attribute, EX l2 : list attribute,
-            PROP ( {{{attrs}}} = l1 ++ l2 )
-                 LOCAL (temp _n (Vint (Int.repr (Zlength l1))); temp _x x; temp _l l)
-                 SEP (attribute_lseg_rep sh l1 l x; attribute_list_rep sh l2 x ))%assert.
-  - Exists l (@nil attribute) (Fset.elements _ attrs).
-  entailer!. unfold attributes_rep, attribute_list_rep. simpl. entailer!.
-  - entailer!.
-  - destruct l2. unfold attribute_list_rep, attribute_lseg_rep at 2. 
-    Intros. rewrite H0 in HRE. contradiction.
-    unfold attribute_list_rep; unfold attribute_lseg_rep at 2; fold attribute_lseg_rep. 
-    Intros r sptr.
+Section Verif.
+  Import db_operations btrees_spec FiniteSet SortedAttributes.
+  Existing Instance db_operations_CompSpecs.
+  Let Gprog := ltac:(with_library prog [attribute_list_length_spec; RL_IsEmpty_spec; RL_CursorIsValid_spec]).
+  Hint Resolve attribute_list_rep_local_facts : saturate_local.
+  Hint Resolve attribute_lseg_rep_local_facts : saturate_local.
+  Hint Resolve attribute_list_rep_valid_pointer : valid_pointer.
+ (*
+  Lemma body_attribute_list_length: semax_body db_operations_Vprog Gprog f_attribute_list_length attribute_list_length_spec.
+  Proof.
+    start_function.
+    forward. forward.
+    forward_loop
+      (EX x : val, EX l1 : list attribute, EX l2 : list attribute,
+                                                   PROP ( {{{attrs}}} = l1 ++ l2 )
+                                                        LOCAL (temp _n (Vint (Int.repr (Zlength l1))); temp _x x; temp _l l)
+                                                        SEP (attribute_lseg_rep sh l1 l x; attribute_list_rep sh l2 x ))%assert.
+    - Exists l (@nil attribute) (Fset.elements _ attrs).
+      entailer!. unfold attributes_rep, attribute_list_rep. simpl. entailer!.
+    - entailer!.
+    - destruct l2. unfold attribute_list_rep, attribute_lseg_rep at 2. 
+      Intros. rewrite H0 in HRE. contradiction.
+      unfold attribute_list_rep; unfold attribute_lseg_rep at 2; fold attribute_lseg_rep. 
+      Intros r sptr.
+      forward.
+      forward.
+      Exists (r, l1 ++ [a], l2). entailer!.
+      split. rewrite semax_lemmas.cons_app in H. rewrite app_assoc in H. auto.
+      rewrite Zlength_app. rewrite Zlength_cons. simpl. reflexivity.
+      unfold attribute_list_rep. cancel.
+      revert l PNl. generalize l1. induction l0; intros. rewrite app_nil_l. simpl. Exists r sptr. entailer.
+      simpl. Intros r0 sptr0. Exists r0 sptr0. entailer!.
+      apply IHl0. auto.
+    - forward. assert (h : l2 = []). rewrite <- H0; easy.
+      subst l2. rewrite app_nil_r in H. subst l1.
+      rewrite Fset.cardinal_spec. rewrite Zlength_correct; auto. entailer!.
+      unfold attributes_rep, attribute_list_rep. sep_apply attribute_lseg_nil. simpl. entailer!.
+  Qed.
+  *)
+  Import btrees btrees_sep Signatures.Cursor.
+  Lemma body_seqscan_next: semax_body db_operations_Vprog Gprog f_seq_scan_next seqscan_next_spec.
+  Proof.
+    unfold seqscan_next_spec, next_spec.
+    start_function.
+    unfold seqscan_iterator, env_assert.
+    destruct e as [rel c], rel as [relnode qrel].
+    Intros qcur.
     forward.
-    forward.
-    Exists (r, l1 ++ [a], l2). entailer!.
-    split. rewrite semax_lemmas.cons_app in H. rewrite app_assoc in H. auto.
-    rewrite Zlength_app. rewrite Zlength_cons. simpl. reflexivity.
-    unfold attribute_list_rep. cancel.
-    revert l PNl. generalize l1. induction l0; intros. rewrite app_nil_l. simpl. Exists r sptr. entailer.
-    simpl. Intros r0 sptr0. Exists r0 sptr0. entailer!.
-    apply IHl0. auto.
-  - forward. assert (h : l2 = []). rewrite <- H0; easy.
-    subst l2. rewrite app_nil_r in H. subst l1.
-    rewrite Fset.cardinal_spec. rewrite Zlength_correct; auto. entailer!.
-    unfold attributes_rep, attribute_list_rep. sep_apply attribute_lseg_nil. simpl. entailer!.
-Qed.
-
+    forward_call ((relnode, qrel), c, qcur, gv).
+    entailer!.
+    unfold fst.
+    forward_if (PROP ( )
+               LOCAL (temp _t'2 (if nat_eq_dec (numKeys relnode) 0%nat then Vint (Int.repr 1) else
+                                       (Val.of_bool (negb (isValid c (relnode, qrel)))));
+                temp _c qcur; gvars gv; temp _env p)
+     SEP (mem_mgr gv; relation_rep (relnode, qrel) (get_numrec (relnode, qrel));
+     cursor_rep c (relnode, qrel) qcur;
+     iter_sepcon (fun x : tuple * val => let (t, p0) := x in tuple_rep Tsh t p0)
+                 (combine (collection it) (map Vint (snd (split (abs_node relnode)))));
+               data_at Tsh t_seq_scan_env (qrel, qcur) p)).
+    forward. entailer!.
+    destruct (nat_eq_dec (numKeys relnode) 0%nat). reflexivity.
+    apply typed_true_tint_Vint in H5. contradiction.
+    forward_call ((relnode, qrel), c, qcur, get_numrec (relnode, qrel)).
+    forward. destruct (nat_eq_dec (numKeys relnode) 0%nat); apply typed_false_tint_Vint in H5.
+    easy. entailer!. destruct btrees.isValid; easy.
+    forward_if. 
+    + forward. Exists (Vint (Int.repr 0)).
+    unfold seqscan_iterator, env_next, env_assert, result_rep.
+    entailer!. Exists qcur.
+    entailer!.
+    - split.
+      * case_eq (next it); intros res next_c heq. unfold snd at 2 3.
+        rewrite (next_collection _ _ H heq).
+        rewrite Forall_forall. intros [t v] htv hc.
+        unfold snd at 1 in hc. unfold fst at 2.
+        Print Rcd.
+        About Signatures.iter.
+        apply Forall_impl with (P := fun x : tuple * val =>
+          option_map Vint (getCRecord c) = Some (snd x) -> fst (next it) = Signatures.Result (fst x)).
+        rewrite heq. destruct a. simpl.
+        intros himpl hnextcur.
+        Print moveToNext.
+      * 
+  Admitted.  
+End Verif.
